Tree simulation and bisimulation

models/oalts/Tree.v
@@ -1,5 +1,6 @@
 Require Import oalts.AsyncEvents.
 Require Import oalts.Sig.
+Require Import models.Sets.
 From Paco Require Import paco.
 
 Module Tree. (* <: Category. *)
@@ -25,57 +26,92 @@ Module Tree. (* <: Category. *)
     intros A t. destruct t as [[X step k]]. reflexivity.
   Qed.
 
-  (* R comes before p, q for paco compatibility *)
-  Definition simF {A B : Type} (f : m A B)
-    (R : tree A -> tree B -> Prop) (p : tree A) (q : tree B) : Prop :=
-    match observe p, observe q with
-    |  @StepF _ _ X step_p k_p, @StepF _ _ X' step_q k_q =>
-      forall x,
-        match f (step_p x) with
-        | 'ev' => exists x', step_q x' = ev' /\ R (k_p x) (k_q x')
-        | τ => R (k_p x) q
-        end
-    end.
+  Section Simulation.
+    Definition simF {A B : Type} (f : m A B)
+      (R : tree A -> tree B -> Prop) (p : tree A) (q : tree B) : Prop :=
+      match observe p, observe q with
+      |  @StepF _ _ X step_p k_p, @StepF _ _ X' step_q k_q =>
+        forall x,
+          match f (step_p x) with
+          | 'ev' => exists x', step_q x' = ev' /\ R (k_p x) (k_q x')
+          | τ => R (k_p x) q
+          end
+      end.
 
-  Lemma simF_mon {A B : Type} (f : m A B) : monotone2 (simF f).
-  Proof.
-    unfold monotone2, simF. intros p q R R' H LE.
-    destruct (observe p) as [X step_p k_p].
-    destruct (observe q) as [X' step_q k_q].
-    intros x. specialize (H x).
-    destruct (f (step_p x)) as [ev' |].
-    - destruct H as [x' [Heq HR]]. exists x'. split; auto.
-    - apply LE. exact H.
-  Qed.
+    Lemma simF_mon {A B : Type} (f : m A B) : monotone2 (simF f).
+    Proof.
+      unfold monotone2, simF. intros p q R R' H LE.
+      destruct (observe p) as [X step_p k_p].
+      destruct (observe q) as [X' step_q k_q].
+      intros x. specialize (H x).
+      destruct (f (step_p x)) as [ev' |].
+      - destruct H as [x' [Heq HR]]. exists x'. split; auto.
+      - apply LE. exact H.
+    Qed.
+
+    Hint Resolve simF_mon : paco.
+
+    Definition sim {A B : Type} (f : m A B) : tree A -> tree B -> Prop :=
+      paco2 (simF f) bot2.
+
+    Proposition simF_sim : forall {A B : Type} (f : m A B) (p : tree A) (q : tree B),
+      simF f (sim f) p q -> sim f p q.
+    Proof.
+      intros A B f p q H. pfold. unfold simF in *.
+      destruct (observe p) as [X step_p k_p].
+      destruct (observe q) as [X' step_q k_q].
+      intros x. specialize (H x).
+      destruct (f (step_p x)) as [ev' |].
+      - destruct H as [x' [Heq HR]]. exists x'. split; auto.
+      - left. exact H.
+    Qed.
+
+    Proposition sim_simF : forall {A B : Type} (f : m A B) (p : tree A) (q : tree B),
+      sim f p q -> simF f (sim f) p q.
+    Proof.
+      intros A B f p q H. punfold H. unfold simF in *.
+      destruct (observe p) as [X step_p k_p].
+      destruct (observe q) as [X' step_q k_q].
+      intros x. specialize (H x).
+      destruct (f (step_p x)) as [ev' |].
+      - destruct H as [x' [Heq HR]]. exists x'. split; auto.
+        destruct HR; auto. contradiction.
+      - destruct H; auto. contradiction.
+    Qed.
+  End Simulation.
 
   #[export] Hint Resolve simF_mon : paco.
 
-  Definition sim {A B : Type} (f : m A B) : tree A -> tree B -> Prop :=
-    paco2 (simF f) bot2.
+  Section Bisimulation.
+    Definition bisimF {A : Type}
+      (R : tree A -> tree A -> Prop) (p : tree A) (q : tree A) : Prop :=
+      match observe p, observe q with
+      |  @StepF _ _ X step_p k_p, @StepF _ _ X' step_q k_q =>
+        (forall x, exists x', step_p x = step_q x' /\ R (k_p x) (k_q x')) /\
+        (forall x', exists x, step_p x = step_q x' /\ R (k_p x) (k_q x'))
+      end.
 
-  Proposition simF_sim : forall {A B : Type} (f : m A B) (p : tree A) (q : tree B),
-    simF f (sim f) p q -> sim f p q.
-  Proof.
-    intros A B f p q H. pfold. unfold simF in *.
-    destruct (observe p) as [X step_p k_p].
-    destruct (observe q) as [X' step_q k_q].
-    intros x. specialize (H x).
-    destruct (f (step_p x)) as [ev' |].
-    - destruct H as [x' [Heq HR]]. exists x'. split; auto.
-    - left. exact H.
-  Qed.
+    Lemma bisimF_mon {A : Type} : monotone2 (@bisimF A).
+    Proof.
+      unfold monotone2, bisimF. intros p q R R' H LE.
+      destruct (observe p) as [X step_p k_p].
+      destruct (observe q) as [X' step_q k_q].
+      destruct H as [Hfw Hbw]; split.
+      - intros x. specialize (Hfw x).
+        destruct Hfw as [x' [Heq Hr]].
+        exists x'. split. 2: apply LE. 
+        all: assumption. 
+      - intros x'. specialize (Hbw x').
+        destruct Hbw as [x [Heq Hr]].
+        exists x. split. 2: apply LE. 
+        all: assumption.
+    Qed.
 
-  Proposition sim_simF : forall {A B : Type} (f : m A B) (p : tree A) (q : tree B),
-    sim f p q -> simF f (sim f) p q.
-  Proof.
-    intros A B f p q H. punfold H. unfold simF in *.
-    destruct (observe p) as [X step_p k_p].
-    destruct (observe q) as [X' step_q k_q].
-    intros x. specialize (H x).
-    destruct (f (step_p x)) as [ev' |].
-    - destruct H as [x' [Heq HR]]. exists x'. split; auto.
-      destruct HR; auto. contradiction.
-    - destruct H; auto. contradiction.
-  Qed.
+    Hint Resolve bisimF_mon : paco.
+
+    Definition bisim {A : Type} : tree A -> tree A -> Prop :=
+      paco2 (bisimF) bot2.
+
+  End Bisimulation.
 
 End Tree.
